theories/max_all_logits.v
@@ -1,27 +1,26 @@
-From Coq Require Import Floats Sint63 Uint63 QArith Lia List PArray.
+From Coq Require Import Floats Sint63 Uint63 QArith Lia List PArray Derive.
 From NeuralNetInterp.Torch Require Import Tensor Einsum Slicing.
 From NeuralNetInterp Require Import max_parameters max max_heuristics.
-From NeuralNetInterp.Util Require Import Pointed.
+From NeuralNetInterp.Util Require Import Pointed ValueExtraction.
 From NeuralNetInterp.Util.Arith Require Import Classes Instances FloatArith.
 Local Open Scope uint63_scope.
 Local Open Scope core_scope.
 
+Local Notation prea := (logits all_tokens) (only parsing).
+Local Notation prev := (PArray.concretize prea) (only parsing).
+Local Definition pre := prev.
+
 Set NativeCompute Timing.
 (*Set NativeCompute Profiling.*)
 (* expected: about 45 minutes in vm, about 19 minutes in native *)
-Time Definition all_tokens_logits_concrete : PArray.concrete_tensor _ _
-  := Eval native_compute in PArray.concretize (logits all_tokens(*.[:82,:]*)).
-(*
-native_compute: Conversion to native code done in 0.00011
-native_compute: Compilation done in 0.36763
-native_compute: Evaluation done in 540.73917
-native_compute: Reification done in 0.29805
-all_tokens_logits_concrete is defined
+Time Local Definition all_tokens_logits_concrete_value := native_compute pre.
 
-Finished transaction in 542.823 secs (541.953u,0.231s) (successful)
-*)
-(*
-Time Definition all_tokens_logits_concrete_vm : PArray.concrete_tensor _ _
-  := Eval vm_compute in PArray.concretize (logits all_tokens).
-*)
-Definition all_tokens_logits : tensor _ _ := PArray.abstract all_tokens_logits_concrete.
+Definition all_tokens_logits_concrete : PArray.concrete_tensor _ _ := extract all_tokens_logits_concrete_value.
+Definition all_tokens_logits_concrete_eq : all_tokens_logits_concrete = prev := extract_eq all_tokens_logits_concrete_value.
+
+Definition all_tokens_logits : tensor _ _ := PArray.reabstract prea all_tokens_logits_concrete.
+Lemma all_tokens_logits_eq idxs : all_tokens_logits idxs = prea idxs.
+Proof.
+  cbv [all_tokens_logits].
+  apply PArray.reabstract_ext_correct, all_tokens_logits_concrete_eq.
+Qed.
